SimSIR compiles

specIR/SimSIR.v
@@ -142,9 +142,9 @@ Inductive _sim_itr (sim_itr: itr_src -> itr_tgt -> Prop): itr_src -> itr_tgt -> 
              (Vis (subevent _ (ICall fname oh_src m vs)) k_src)
              (Vis (subevent _ (ICall fname oh_tgt m vs)) k_tgt)
 | sim_ecall
-    sg m vs
-    fptr_src oh_src k_src
-    fptr_tgt oh_tgt k_tgt
+    sg m vs fptr
+    oh_src k_src
+    oh_tgt k_tgt
     (O: SO oh_src oh_tgt)
     (SIM: HProper (SALL **> sim_itr) k_src k_tgt)
     (* (SIM: forall *)
@@ -154,8 +154,8 @@ Inductive _sim_itr (sim_itr: itr_src -> itr_tgt -> Prop): itr_src -> itr_tgt -> 
     (*     sim_itr (k_src (ohr_src, (mr, vr))) (k_tgt (ohr_tgt, (mr, vr)))) *)
   :
     _sim_itr sim_itr
-             (Vis (subevent _ (ECall sg fptr_src oh_src m vs)) k_src)
-             (Vis (subevent _ (ECall sg fptr_tgt oh_tgt m vs)) k_tgt)
+             (Vis (subevent _ (ECall sg fptr oh_src m vs)) k_src)
+             (Vis (subevent _ (ECall sg fptr oh_tgt m vs)) k_tgt)
 | sim_nb
     i_src k_tgt
   :
@@ -163,7 +163,7 @@ Inductive _sim_itr (sim_itr: itr_src -> itr_tgt -> Prop): itr_src -> itr_tgt -> 
 | sim_ub
     k_src i_tgt
   :
-    _sim_itr sim_itr (Vis (subevent _ (ENB)) k_src) i_tgt
+    _sim_itr sim_itr (Vis (subevent _ (EUB)) k_src) i_tgt
 | sim_choose_src
     X_src
     k_src i_tgt
@@ -171,14 +171,15 @@ Inductive _sim_itr (sim_itr: itr_src -> itr_tgt -> Prop): itr_src -> itr_tgt -> 
   :
     _sim_itr sim_itr
              (Vis (subevent _ (EChoose X_src)) k_src)
-             (Tau i_tgt)
+             (Tau (Tau i_tgt))
 | sim_choose_tgt
     X_tgt
     k_tgt i_src
     (SIM: forall x_tgt, sim_itr i_src (k_tgt x_tgt))
+    (INHAB: inhabited X_tgt)
   :
     _sim_itr sim_itr
-             (Tau i_src)
+             (Tau (Tau i_src))
              (Vis (subevent _ (EChoose X_tgt)) k_tgt)
 .
 
@@ -309,15 +310,15 @@ Inductive _sim_st (sim_st: st_src -> st_tgt -> Prop): st_src -> st_tgt -> Prop :
   :
     _sim_st sim_st (Tau i_src) (Tau i_tgt)
 | sim_st_ecall
-    sg m vs
-    fptr_src oh_src k_src
-    fptr_tgt oh_tgt k_tgt
+    sg m vs fptr
+    oh_src k_src
+    oh_tgt k_tgt
     (O: SO oh_src oh_tgt)
     (SIM: HProper (SALL **> sim_st) k_src k_tgt)
   :
     _sim_st sim_st
-             (Vis (subevent _ (ECall sg fptr_src oh_src m vs)) k_src)
-             (Vis (subevent _ (ECall sg fptr_tgt oh_tgt m vs)) k_tgt)
+             (Vis (subevent _ (ECall sg fptr oh_src m vs)) k_src)
+             (Vis (subevent _ (ECall sg fptr oh_tgt m vs)) k_tgt)
 | sim_st_nb
     i_src k_tgt
   :
@@ -325,7 +326,7 @@ Inductive _sim_st (sim_st: st_src -> st_tgt -> Prop): st_src -> st_tgt -> Prop :
 | sim_st_ub
     k_src i_tgt
   :
-    _sim_st sim_st (Vis (subevent _ (ENB)) k_src) i_tgt
+    _sim_st sim_st (Vis (subevent _ (EUB)) k_src) i_tgt
 | sim_st_choose_src
     X_src
     k_src i_tgt
@@ -333,14 +334,15 @@ Inductive _sim_st (sim_st: st_src -> st_tgt -> Prop): st_src -> st_tgt -> Prop :
   :
     _sim_st sim_st
             (Vis (subevent _ (EChoose X_src)) k_src)
-            i_tgt 
+            (Tau i_tgt)
 | sim_st_choose_tgt
     X_tgt
     k_tgt i_src
+    (INHAB: inhabited X_tgt)
     (SIM: forall x_tgt, sim_st i_src (k_tgt x_tgt))
   :
     _sim_st sim_st
-            i_src
+            (Tau i_src)
             (Vis (subevent _ (EChoose X_tgt)) k_tgt)
 .
 
@@ -366,44 +368,47 @@ Hint Resolve sim_st_mon: paco.
 
 
 
+Section SIM.
 
-Lemma sim_prog_sim_st_aux
-      p_src p_tgt
-      (SIMP: sim_prog p_src p_tgt)
-      i_src i_tgt
-      (SIM: sim_itr i_src i_tgt)
-  :
-    sim_st (interp_mrec (interp_function p_src) i_src) (interp_mrec (interp_function p_tgt) i_tgt)
-.
-Proof.
-  revert_until SIMP.
-  ginit.
-  { intros. eapply cpn2_wcompat; et. eauto with paco. }
-  gcofix CIH.
-  i. rewrite ! unfold_interp_mrec.
-  punfold SIM. inv SIM; cbn.
-  - gstep. econs; et.
-  - pclearbot. gstep. econs; et. gbase. et.
-  - pclearbot. gstep. econs; et. gbase.
-    eapply CIH. eapply sim_itr_bind.
-    { u. ii. repeat spc SIM0. pclearbot. eauto. }
-    hexploit (SIMP fname); et. intro T.
-    inv T.
-    { pfold. econs; et. }
-    exploit H1; et.
-  - gstep. econs; et. u in *. gstep. econs; et. repeat spc SIM0. des; ss. gbase. eapply CIH.
-    eauto with paco.
-  - gstep. econs; et.
-  - gstep. econs; et.
-  - gstep. des. pclearbot. econs; et. esplits; et. gstep. econs; et. eauto with paco.
-  - gstep. pclearbot. econs; et. ii. repeat spc SIM0.
-    gstep. econs; et. eauto with paco.
-Qed.
+  Variable p_src: program owned_heap_src.
+  Variable p_tgt: program owned_heap_tgt.
+  Hypothesis (SIMP: sim_prog p_src p_tgt).
 
-Theorem sim_prog_sim_st
-        p_src p_tgt
-        (SIMP: sim_prog p_src p_tgt)
-  :
+  Lemma sim_prog_sim_st
+        i_src i_tgt
+        (SIM: sim_itr i_src i_tgt)
+    :
+      sim_st (interp_mrec (interp_function p_src) i_src)
+             (interp_mrec (interp_function p_tgt) i_tgt)
+  .
+  Proof.
+    revert_until SIMP.
+    ginit.
+    { intros. eapply cpn2_wcompat; et. eauto with paco. }
+    gcofix CIH.
+    i. rewrite ! unfold_interp_mrec.
+    punfold SIM. inv SIM; cbn.
+    - gstep. econs; et.
+    - pclearbot. gstep. econs; et. gbase. et.
+    - pclearbot. gstep. econs; et. gbase.
+      eapply CIH. eapply sim_itr_bind.
+      { u. ii. repeat spc SIM0. pclearbot. eauto. }
+      hexploit (SIMP fname); et. intro T.
+      inv T.
+      { pfold. econs; et. }
+      exploit H1; et.
+    - gstep. econs; et. u in *. gstep. econs; et. repeat spc SIM0. des; ss. gbase. eapply CIH.
+      eauto with paco.
+    - gstep. econs; et.
+    - gstep. econs; et.
+    - gstep. des. pclearbot. econs; et. esplits; et. gstep.
+      rewrite (unfold_interp_mrec _ (Tau i_tgt0)). cbn. econs; et. eauto with paco.
+    - gstep. pclearbot. econs; et. ii. repeat spc SIM0. gstep.
+      rewrite (unfold_interp_mrec _ (Tau i_src0)). cbn. econs; et. eauto with paco.
+  Qed.
+
+  (*** The result that we wanted -- allows reasoning each function "locally" and then compose ***)
+  Theorem adequacy_local_local:
     forall
       (fname: ident) m vs oh_src oh_tgt
       (O: SO oh_src oh_tgt)
@@ -411,105 +416,41 @@ Theorem sim_prog_sim_st
       (<<SIM: sim_st (interp_program0 p_src (ICall fname oh_src m vs))
                      (interp_program0 p_tgt (ICall fname oh_tgt m vs))
                      >>)
-.
-Proof.
-  {
-    ii.
-    eapply sim_prog_sim_st_aux; ss.
-    hexploit (SIMP fname); et. intro T. inv T; ss.
-    { pfold. econs; et. }
-    repeat (spc H1). des. ss.
-  }
-Qed.
-
-
-(*** sim fn / program ***)
-(* Let fn_src := InternalCallE owned_heap_src ~> SIRmini.state. *)
-(* Let fn_tgt := InternalCallE owned_heap_tgt ~> SIRmini.state. *)
-
-(* Definition sim_fn (k_src: fn_src) (k_tgt: fn_tgt): Prop := forall *)
-(*     fname m vs *)
-(*     oh_src oh_tgt *)
-(*     (O: SO oh_src oh_tgt) *)
-(*   , *)
-(*     <<SIM: sim_st (k_src _ (ICall fname oh_src m vs)) (k_tgt _ (ICall fname oh_tgt m vs))>> *)
-(* . *)
-Let fn_src := function owned_heap_src.
-Let fn_tgt := function owned_heap_tgt.
-
-Definition sim_fn (k_src: fn_src) (k_tgt: fn_tgt): Prop := forall
-    m vs
-    oh_src oh_tgt
-    (O: SO oh_src oh_tgt)
-  ,
-    <<SIM: sim_st (k_src oh_src m vs) (k_tgt oh_tgt m vs)>>
-.
-
-Definition sim_prog (p_src: program owned_heap_src) (p_tgt: program owned_heap_tgt): Prop :=
-  (eq ===> 
-.
-Definition sim_prog (p_src: program owned_heap_src) (p_tgt: program owned_heap_tgt): Prop :=
-  forall fname, <<SIM: option_rel sim_fn (p_src fname) (p_tgt fname)>>
-.
-
-Theorem sim_prog_sim_st
-        p_src p_tgt
-        (SIM: sim_prog p_src p_tgt)
-  :
-    <<SIM: sim_ktr (interp_program0 p_src) (interp_program0 p_tgt)>>
-.
-Proof.
-Qed.
-Global Instance eq_itree_mrec:
-  Proper (sim_prog ==> eq ==> sim_st) (interp_program0).
-Proof.
-  ginit. gcofix CIH. intros.
-  rewrite !unfold_interp_mrec.
-  punfold H0. inv H0; try discriminate; pclearbot; simpobs; [| |destruct e]; gstep.
-  - apply reflexivity.
-  - econstructor. eauto with paco.
-  - econstructor. gbase. eapply CIH. apply eqit_bind; auto; reflexivity.
-  - econstructor. gstep; constructor. auto with paco.
-Qed.
-
-Theorem sim_sim
-        
-
-
-
-
-
-
-
-
-
-
-
-
-
-
-Section SMO.
-
-  Record t: Type :=
-    mk {
-      sm :> SimMem.t;
-      oh_src: Any;
-      oh_tgt: Any;
+  .
+  Proof.
+    {
+      ii.
+      eapply sim_prog_sim_st; ss.
+      hexploit (SIMP fname); et. intro T. inv T; ss.
+      { pfold. econs; et. }
+      repeat (spc H1). des. ss.
     }
-  .
+  Qed.
 
-  Inductive wf (smo: t): Prop :=
-  | wf_intro
-      (oh_src: owned_heap_src) (oh1: owned_heap1)
-      (MWF: SimMem.wf smo)
-      (OHSRC: smo.(oh_src) = upcast oh_src)
-      (OHTGT: smo.(oh_tgt) = upcast oh1)
-  .
+  (*** lifting above proof into small-step semantics ***)
+  Section SMO.
 
-  Local Obligation Tactic := try (by ii; des; ss).
+    Record t: Type :=
+      mk {
+          sm :> SimMem.t;
+          oh_src: Any;
+          oh_tgt: Any;
+        }
+    .
 
-  Program Instance SimMemOh: (SimMemOh.class) :=
-    {|
+    Inductive wf (smo: t): Prop :=
+    | wf_intro
+        (o_src: owned_heap_src) (o_tgt: owned_heap_tgt)
+        (MWF: SimMem.wf smo)
+        (OHSRC: smo.(oh_src) = upcast o_src)
+        (OHTGT: smo.(oh_tgt) = upcast o_tgt)
+        (O: SO o_src o_tgt)
+    .
+
+    Local Obligation Tactic := try (by ii; des; ss).
+
+    Program Instance SimMemOh: (SimMemOh.class) :=
+      {|
       SimMemOh.t := t;
       SimMemOh.sm := sm;
       SimMemOh.oh_src := oh_src;
@@ -519,184 +460,191 @@ Section SMO.
       SimMemOh.lepriv := SimMem.lepriv;
       SimMemOh.midx := Some mi;
       SimMemOh.set_sm := fun smo sm => mk sm smo.(oh_src) smo.(oh_tgt);
-    |}
-  .
-  Next Obligation.
-    ii. eapply PR.
-  Qed.
-  Next Obligation.
-    ii. inv WF.
-    econs; ss; et.
-  Qed.
-  Next Obligation.
-    ss. ii. destruct smo_src; ss.
-  Qed.
-
-End SMO.
-
-
-
-Variable p_src: program owned_heap_src.
-Variable p1: program owned_heap1.
-Variable ioh_src: SkEnv.t -> owned_heap_src.
-Variable ioh1: SkEnv.t -> owned_heap1.
-Hypothesis (SIMP: sim_prog p_src p1).
-Hypothesis (SIMO: forall skenv, SO (ioh_src skenv) (ioh1 skenv)).
-Variable sk: Sk.t.
-Let md_src: Mod.t := (SIRmini.module sk p_src mi ioh_src).
-Let md_tgt: Mod.t := (SIRmini.module sk p1 mi ioh1).
-
-
-
-(*** Lifting to SimModSem ***)
-Section SIMMODSEM.
-
-Variable skenv_link: SkEnv.t.
-Variable sm_link: SimMem.t.
-Let ms_src: ModSem.t := (Mod.modsem md_src skenv_link).
-Let ms_tgt: ModSem.t := (Mod.modsem md_tgt skenv_link).
-Hypothesis (INCL: SkEnv.includes skenv_link (Mod.sk md_src)).
-Hypothesis (WF: SkEnv.wf skenv_link).
-
-Local Existing Instance SimMemOh.
-Local Arguments ModSemPair.mk [SM] [SS] _ _ _ _ [SMO].
-
-Definition msp: ModSemPair.t := ModSemPair.mk (md_src skenv_link) (md_tgt skenv_link)
-                                              (SimSymbId.mk md_src md_tgt) sm_link.
-
-Inductive match_states (idx: nat): SIRmini.state owned_heap_src ->
-                                   SIRmini.state owned_heap1 -> SimMemOh.t -> Prop :=
-| match_states_intro
-    st_src st1 smo_src
-    fid m vs oh_src oh1
-    (O: SO oh_src oh1)
-    (ST_src: st_src = (interp_program_src p_src (ICall fid oh_src m vs)))
-    (ST1: st1 = (interp_program_src p1 (ICall fid oh1 m vs)))
-    (MWF: SimMemOh.wf smo_src)
-  :
-    match_states idx st_src st1 smo_src
-.
-
-(*** TODO: move to SIRCommon2 ***)
-Lemma unfold_interp_mrec :
-forall (D E : Type -> Type) (ctx : forall T : Type, D T -> itree (D +' E) T) 
-  (R : Type) (t : itree (D +' E) R), interp_mrec ctx t = _interp_mrec ctx (observe t).
-Proof.
-  i. f. eapply unfold_interp_mrec; et.
-Qed.
-
-Lemma match_states_lxsim
-      idx st_src_src st_tgt_src smo_src
-      (MATCH: match_states idx st_src_src st_tgt_src smo_src)
-  :
-    <<XSIM: lxsim (md_src skenv_link) (md_tgt skenv_link)
-                  (fun _ => () -> exists (_ : ()) (_ : mem), True)
-                  (Ord.lift_idx lt_wf idx) st_src_src st_tgt_src smo_src>>
-.
-Proof.
-  revert_until idx. revert idx.
-  pcofix CIH. i. pfold.
-  ii. clear SUSTAR.
-
-  inv MATCH. ss.
-  hexploit (SIMP fid); et. intro R.
-  unfold interp_program_src, mrec in *.
-  (* f in ST_src. rewrite unfold_interp_mrec in ST_src. ss. *)
-  inv R; des_ifs; ss.
-  { des_ifs. rewrite ! unfold_interp_mrec. ss. econs 2; eauto. ii. econs 3; et.
-    { ss. ii. inv STEPTGT; ss. }
-    { esplits; ss; et. by (econs; ss). }
-  }
-  des_ifs.
-  rename H1 into SK.
-  exploit (SK m vs); et. intro SI. des.
-  rewrite ! unfold_interp_mrec. rename f_src into f1. rename f into f_src.
-  punfold SI. inv SI.
-  - (* RET *)
-    econstructor 4 with (smo_ret := mk (SimMemId.mk m_src m_src) (upcast oh2) (upcast oh3)); ss; eauto.
-    { econs; ss; et. }
-    { econs; ss; et. }
-    { econs; ss; et. }
-    { rr. esplits; ss; et. econs; ss; et. }
-  - (* TAU *)
-    econs 1; ss; et. ii. clear SU.
-    econs 1; ss; et; swap 2 3.
-    { split; intro T; rr in T; des; ss; inv T; ss. }
-    { eapply modsem_receptive; et. }
-    ii. inv STEPSRC; ss; clarify. esplits; ss; et.
-    { left. apply plus_one. econs; ss; et.
-      { eapply modsem_determinate; ss; et. }
+      |}
+    .
+    Next Obligation.
+      ii. eapply PR.
+    Qed.
+    Next Obligation.
+      ii. inv WF.
       econs; ss; et.
-    }
-    right. eapply CIH. econs; ss; et.
-Qed.
+    Qed.
+    Next Obligation.
+      ss. ii. destruct smo0; ss.
+    Qed.
+
+  End SMO.
+
+  Variable ioh_src: SkEnv.t -> owned_heap_src.
+  Variable ioh_tgt: SkEnv.t -> owned_heap_tgt.
+  Hypothesis (SIMO: forall skenv, SO (ioh_src skenv) (ioh_tgt skenv)).
+  Variable sk: Sk.t.
+  Let md_src: Mod.t := (SIRmini.module sk p_src mi ioh_src).
+  Let md_tgt: Mod.t := (SIRmini.module sk p_tgt mi ioh_tgt).
 
 
 
-End SIMMODSEM.
+  (*** Lifting to SimModSem ***)
+  Section SIMMODSEM.
 
-Theorem sim_mod
-        p_src p1
-        ioh_src ioh1
-        (SIMP: sim_prog p_src p1)
-        (SIMO: forall skenv, SO (ioh_src skenv) (ioh1 skenv))
-  :
-    forall sk,
-      ModPair.sim (SimSymbId.mk_mp (SIRmini.module sk p_src mi ioh_src) (SIRmini.module sk p1 mi ioh1))
-.
-Proof.
-  ii. econs; ss; eauto.
-  ii. esplits; ss; et. econs; ss; et.
-Qed.
+    Variable skenv_link: SkEnv.t.
+    Variable sm_link: SimMem.t.
+    Let ms_src: ModSem.t := (Mod.modsem md_src skenv_link).
+    Let ms_tgt: ModSem.t := (Mod.modsem md_tgt skenv_link).
+    Hypothesis (INCL: SkEnv.includes skenv_link (Mod.sk md_src)).
+    Hypothesis (WF: SkEnv.wf skenv_link).
+
+    Local Existing Instance SimMemOh.
+    Local Arguments ModSemPair.mk [SM] [SS] _ _ _ _ [SMO].
+
+    Definition msp: ModSemPair.t := ModSemPair.mk (md_src skenv_link) (md_tgt skenv_link)
+                                                  (SimSymbId.mk md_src md_tgt) sm_link.
+
+    Inductive match_states (idx: nat): SIRmini.state owned_heap_src ->
+                                       SIRmini.state owned_heap_tgt -> SimMemOh.t -> Prop :=
+    | match_states_intro
+        st_src st_tgt smo0
+        (SIM: sim_st st_src st_tgt)
+        (MWF: SimMemOh.wf smo0)
+      :
+        match_states idx st_src st_tgt smo0
+    .
+
+    Lemma match_states_lxsim
+          idx st_src_src st_tgt_src smo_src
+          (MATCH: match_states idx st_src_src st_tgt_src smo_src)
+      :
+        <<XSIM: lxsim (md_src skenv_link) (md_tgt skenv_link)
+                      (fun _ => () -> exists (_ : ()) (_ : mem), True)
+                      (Ord.lift_idx lt_wf idx) st_src_src st_tgt_src smo_src>>
+    .
+    Proof.
+      revert_until idx. revert idx.
+      ginit.
+      { intros. eapply cpn4_wcompat; eauto with paco. }
+      gcofix CIH. i. gstep.
+      ii. clear SUSTAR.
+
+      inv MATCH. ss.
+      punfold SIM. inv SIM.
+      - assert(U:=MWF).
+        inv MWF. inv MWF0. destruct smo_src; ss. destruct sm0; ss. clarify.
+        econstructor 4 with (smo_ret := mk (SimMemId.mk m m)
+                                           (upcast oh_src0) (upcast oh_tgt0)); ss; eauto.
+        + econs; ss; et.
+        + econs; ss; et.
+        + econs; ss; et.
+        + rr. ss. esplits; ss; et.
+          { econs; ss; et. }
+      - (* TAU *)
+        econs 1; et.
+        econs 1; et; swap 2 3.
+        { split; intro T; rr in T; des; ss; inv T; ss. }
+        { eapply modsem_receptive; et. }
+        ii; ss. inv STEPSRC; ss. clarify. esplits; ss; et.
+        { left. eapply plus_one. rr. esplits; et.
+          { eapply modsem_determinate; ss; et. }
+          econs; et.
+        }
+        pclearbot. gbase. eapply CIH. econs; et.
+      - (* ECALL *)
+        econs 3; et.
+        { admit "TODO: fix -- ~step, ~ret should suffice". }
+        ii; ss. inv ATSRC. csc.
+        eexists _, _, (mk (SimMemId.mk m0 m0) (upcast oh_src1) (upcast oh_tgt0)); ss.
+        esplits; ss; et.
+        { rr. ss. esplits; ss; et. econs; ss; et. }
+        { econs; ss; et. }
+        { econs; ss; et. }
+        ii. des. inv AFTERSRC; ss. inv GETK; ss. csc.
+        rename oh_src0 into oh_src1.
+        rename _oh0 into oh_src0.
+        rr in SIMRETV. des; ss. inv SIMRETV0; ss. clarify.
+        inv MWF0. ss. destruct smo_ret; ss. destruct sm0; ss. subst. clarify. clear_tac.
+        esplits; et.
+        { econs; ss; et. econs; ss; et. }
+        u in SIM0.
+        hexploit SIM0; et.
+        { instantiate (2:= (o_src, (_, _))). instantiate (1:= (o_tgt, (_, _))). ss. }
+        intro T. des; ss.
+        gbase. eapply CIH. econs; et.
+      - (* NB *)
+        econs 2; ss; et. ii.
+        econs 3; ss; et.
+        { ii; ss. inv STEPTGT; ss. }
+        { esplits; et. econsby ss. }
+      - (* UB *)
+        econs 2; ss; et. ii.
+        exploit SAFESRC; et.
+        { eapply star_refl. }
+        intro T; des; ss.
+        + rr in EVCALL. des; ss. inv EVCALL; ss.
+        + rr in EVRET. des; ss. inv EVRET; ss.
+        + inv EVSTEP; ss.
+      - (* CHOOSE SRC *)
+        des. pclearbot.
+        econs 2; ss; et. ii.
+        econs 1; ss; et; cycle 1.
+        { esplits; ss; et. econs; ss; et. }
+        { ii. inv STEPTGT; ss; clarify. esplits; et.
+          + left. eapply plus_one. econs 3; ss; et.
+          + gbase. eapply CIH. econs; et.
+        }
+      - (* CHOOSE TGT *)
+        des. pclearbot. inv INHAB.
+        econs 2; ss; et. ii.
+        econs 1; ss; et; cycle 1.
+        { esplits; ss; et. econs 3; ss; et. }
+        { ii. inv STEPTGT; ss; csc. esplits; et.
+          + left. eapply plus_one. econs; ss; et.
+          + gbase. eapply CIH. econs; et.
+        }
+    Unshelve.
+      all: ss.
+      all: try (econsby ss).
+    Qed.
+
+    Theorem sim_modsem: ModSemPair.sim msp.
+    Proof.
+      econstructor 1 with (sidx := unit) (sound_states := top4); eauto;
+        try apply SoundTop.sound_state_local_preservation; et; try (by ii; ss).
+      { ii. eapply Preservation.local_preservation_noguarantee_weak.
+        apply SoundTop.sound_state_local_preservation; et.
+      }
+      { ii. ss. eexists (mk _ _ _); ss. esplits; eauto. econs; ss; eauto. }
+      ii. ss. esplits; eauto.
+      - ii. des. inv INITTGT. inv SAFESRC. ss. des_ifs_safe.
+        esplits; eauto.
+        { econs; ss; et. }
+        eapply match_states_lxsim; eauto.
+        econs; ss; et.
+        eapply sim_prog_sim_st; et.
+        rr in SIMARGS. des. inv SIMARGS0; ss. clarify. inv MWF. ss. destruct sm_arg; ss.
+        destruct sm0; ss. subst. clarify. clear_tac.
+        assert(fid0 = fid).
+        { apply_all_once Genv.find_invert_symbol. clarify. }
+        clarify.
+        repeat spc SIMP. inv SIMP; ss.
+        { pfold. econs; et. }
+        { eapply H1; et. }
+      - i; des. inv SAFESRC. ss. des_ifs.
+        rr in SIMARGS. des. inv SIMARGS0; ss. clarify. destruct sm_arg; ss. destruct sm0; ss. clarify.
+        esplits; et. econs; ss; et.
+    Unshelve.
+      all: ss.
+      all: try (econsby ss).
+    Qed.
+
+  End SIMMODSEM.
+
+  Theorem sim_mod: ModPair.sim (SimSymbId.mk_mp (SIRmini.module sk p_src mi ioh_src)
+                                                (SIRmini.module sk p_tgt mi ioh_tgt)).
+  Proof.
+    ii. econs; ss; eauto.
+    ii. rr in SIMSKENVLINK. clarify. esplits. eapply sim_modsem; et.
+  Qed.
+
+End SIM.
 
 End OWNEDHEAP.
 
-
-
-
-
-
-
-
-
-
-
-
-
-(*** Relating with SimMem Id ***)
-
-Program Definition boo := SimMem eq eq _.
-Next Obligation.
-  subst. ss.
-Qed.
-
-Require Import SimMemId.
-Lemma SimMem_eta
-      (smc0 smc1: SimMem.class)
-      (EQ0: smc0.(@SimMem.t) = smc1.(@SimMem.t))
-      (EQ1: smc0.(@SimMem.src) ~= smc1.(@SimMem.src))
-      (EQ2: smc0.(@SimMem.ptt_src) ~= smc1.(@SimMem.ptt_src))
-      (EQ3: smc0.(@SimMem.tgt) ~= smc1.(@SimMem.tgt))
-      (EQ4: smc0.(@SimMem.ptt_tgt) ~= smc1.(@SimMem.ptt_tgt))
-      (EQ5: smc0.(@SimMem.wf) ~= smc1.(@SimMem.wf))
-      (EQ6: smc0.(@SimMem.le) ~= smc1.(@SimMem.le))
-      (EQ7: smc0.(@SimMem.lepriv) ~= smc1.(@SimMem.lepriv))
-      (EQ8: smc0.(@SimMem.sim_val) ~= smc1.(@SimMem.sim_val))
-      (EQ9: smc0.(@SimMem.sim_val_list) ~= smc1.(@SimMem.sim_val_list))
-      (EQ10: smc0.(@SimMem.unchanged_on) ~= smc1.(@SimMem.unchanged_on))
-  :
-    smc0 = smc1
-.
-Proof.
-  destruct smc0, smc1; ss.
-  clarify.
-  apply_all_once JMeq_eq. clarify.
-  f_equal; try eapply Axioms.proof_irr.
-Qed.
-
-Goal boo = SimMemId.
-Proof.
-  eapply SimMem_eta; ss.
-Abort.
-  
-(*** Maybe we should define common ancestor, and let SimMemId // SimSIR use the same thing. ***)
